wip pairing

examples/PairingHeap/PairingHeap_proof.v
@@ -21,11 +21,11 @@ License: CC-by 4.0.
 
 *)
 
+(* ********************************************************************** *)
+(* ********************************************************************** *)
+(* ********************************************************************** *)
+(** * General Definitions *)
 
-(* ********************************************************************** *)
-(* ********************************************************************** *)
-(* ********************************************************************** *)
-(** * Representation and lemmas *)
 
 (* ********************************************************************** *)
 (** ** Types of elements *)
@@ -35,6 +35,326 @@ License: CC-by 4.0.
 
 Notation "'elem'" := (int).
 Notation "'elems'" := (multiset elem).
+
+(* ********************************************************************** *)
+(** ** List unions *)
+
+(** [list_union Es] computes the iterated union of the multisets in the list [Es] *)
+
+Definition list_union (Es:list elems) : elems :=
+  LibList.fold_right union \{} Es.
+
+
+(** Normalization lemmas for [list_union] *)
+
+Lemma list_union_nil :
+  list_union (@nil elems) = \{}.
+Proof using. auto. Qed.
+
+Lemma list_union_cons : forall E Es,
+  list_union (E::Es) = E \u list_union Es.
+Proof using. auto. Qed.
+
+(** Hints *)
+
+Hint Rewrite list_union_nil list_union_cons : rew_listx.
+Hint Rewrite (@union_empty_r elems _ _ _) (@union_empty_l elems _ _ _) : rew_listx.
+
+Hint Constructors Forall Forall2 list_sub.
+
+
+(* ********************************************************************** *)
+(** ** Minimal elements *)
+
+(** Auxiliary definition for specifications *)
+
+Definition min_of (E:elems) (x:elem) : Prop :=
+  x \in E /\ forall_ y \in E, x <= y.
+
+(** Auxiliary definition for stating invariants follow. *)
+
+(** [is_ge x] is a predicate that characterizes items no less than [x] *)
+
+Definition is_ge (x y:elem) : Prop :=
+  x <= y.
+
+(** Hints *)
+
+Hint Unfold is_ge.
+Hint Extern 1 (_ < _) => simpl; math.
+Hint Extern 1 (_ <= _) => simpl; math.
+Hint Extern 1 (_ = _ :> multiset _) => rew_listx; multiset_eq.
+Hint Extern 1 (_ \in _) => multiset_in.
+
+(** Lemmas to manipulate the invariant [Forall (foreach (is_ge x)) Es] *)
+
+Lemma Forall_foreach_is_ge_inv : forall x y Es,
+  Forall (foreach (is_ge x)) Es ->
+  y \in list_union Es ->
+  x <= y.
+Proof using.
+  introv M Hy. unfolds list_union. induction M; rew_listx in *.
+  { multiset_in Hy. }
+  { multiset_in Hy. { applys* H. } { applys* IHM. } }
+Qed.
+
+Lemma foreach_list_union : forall P Es,
+  Forall (foreach P) Es ->
+  foreach P (list_union Es).
+Proof using.
+  introv M. induction M.
+  { applys foreach_empty. }
+  { unfold list_union; rew_listx. applys* foreach_union. }
+Qed.
+
+
+
+(* ********************************************************************** *)
+(* ********************************************************************** *)
+(* ********************************************************************** *)
+(** * Alternative Approach, Without a Pure Tree *)
+
+From TLC Require Import LibFix.
+Module Alternative.
+
+
+(* ******************************************************* *)
+(** ** Representation predicates *)
+
+(** [in x Es E] captures the invariant for a node. *)
+
+Definition inv (x:elem) (Es:list elems) (E:elems) : Prop :=
+     Forall (foreach (is_ge x)) Es
+  /\ E = \{x} \u (list_union Es).
+
+(** [q ~> Repr E] is a notation for [Repr E q]. It relates a pointer [q] with the
+    multiset of items that it represents in memory, and enforces invariants.
+    Because it is recursive, we use the optimal fixed point combinator to
+    define [Repr]. We here cheat and axiomatize termination. *)
+
+Definition ReprFunctional (Repr:elems->loc->hprop) (E:elems) (q:loc) : hprop :=
+  \exists (x:elem) (q':loc) (Es:list elems),
+       q ~~~>`{ value' := x; sub' := q' }
+    \* q' ~> MListOf Repr Es
+    \* \[inv x Es E].
+
+Definition Repr := FixFun2 ReprFunctional.
+
+Axiom fix_Repr : forall E q, (* cheating for fixpoint *)
+  Repr E q = ReprFunctional Repr E q.
+
+(** [q ~> Heap E] relates a pointer on a heap [p] with the multiset of items [E]
+    that are stored in the heap. It uses [Contents E c] as an auxiliary definition. *)
+
+Definition Contents (E:elems) (c:contents_) : hprop :=
+  match c with
+  | Empty => \[E = \{}]
+  | Nonempty p => (p ~> Repr E)
+  end.
+
+Definition Heap (E:elems) (p:heap_) : hprop :=
+  \exists c, p ~~> c \* Contents E c.
+
+
+(* ******************************************************* *)
+(** ** Paraphrase definitions as equalities *)
+
+Lemma Contents_eq : forall E c,
+  Contents E c = (match c with
+  | Empty => \[E = \{}]
+  | Nonempty p => (p ~> Repr E)
+  end).
+Proof using. auto. Qed.
+
+Lemma Heap_eq : forall p E,
+  p ~> Heap E = \exists c, p ~~> c \* Contents E c.
+Proof using. auto. Qed.
+
+Lemma Repr_eq : forall q E,
+  q ~> Repr E = \exists (x:elem) (q':loc) (Es:list elems),
+       q ~~~>`{ value' := x; sub' := q' }
+    \* q' ~> MListOf Repr Es
+    \* \[inv x Es E].
+Proof using.
+  intros. xunfold Repr at 1.
+  fold Repr. rewrite fix_Repr. auto.
+Qed.
+
+Lemma Repr_intro : forall q x q' Es,
+  Forall (foreach (is_ge x)) Es ->
+      q ~~~>`{ value' := x; sub' := q' } \* q' ~> MListOf Repr Es
+  ==> q ~> Repr (\{x} \u (list_union Es)).
+Proof using. Hint Unfold inv. intros. xchange* <- (Repr_eq q). Qed.
+
+Arguments Repr_intro : clear implicits.
+
+Lemma haffine_Repr : forall p E,
+  haffine (p ~> Repr E).
+Proof using.
+  admit_goal IH. (* cheating for induction *)
+  set_eq R: Repr in IH.
+  intros. rewrite Repr_eq. xaffine. subst R.
+  applys haffine_MListOf. intros. applys IH.
+Qed.
+
+Hint Resolve haffine_Repr : haffine.
+
+
+(* ******************************************************* *)
+(** ** Lemmas about representation predicates *)
+
+Lemma inv_not_empty : forall x Es E,
+  inv x Es E ->
+  E <> \{}.
+Proof using. introv (I1&I2). subst. multiset_inv. Qed.
+
+Lemma Repr_not_empty : forall q E,
+  q ~> Repr E ==> \[E <> \{}] \* q ~> Repr E.
+Proof using.
+  intros. rewrite Repr_eq. xpull ;=> x q' Es I. lets: inv_not_empty I. xsimpl*.
+Qed.
+
+Lemma Contents_is_empty : forall c E,
+  Contents E c ==> \[c = Empty <-> E = \{}] \* Contents E c.
+Proof using.
+  intros.  unfold Contents. destruct c.
+  { xsimpl*. }
+  { xchange Repr_not_empty ;=> N. xsimpl. iff H; false. }
+Qed.
+
+Lemma Heap_Nonempty : forall p q E,
+  p ~~> Nonempty q \* q ~> Repr E ==> p ~> Heap E.
+Proof using.
+  intros. xchanges Repr_not_empty ;=> N. xunfold Heap. xsimpl.
+Qed.
+
+Lemma Heap_Empty : forall p,
+  p ~~> Empty ==> p ~> Heap \{}.
+Proof using. intros. xunfold Heap. unfold Contents. xsimpl*. Qed.
+
+
+(* ******************************************************* *)
+(** ** Verification *)
+
+Lemma Triple_create :
+  SPEC (create tt)
+    PRE \[]
+    POST (fun p => p ~> Heap \{}).
+Proof using.
+  xcf. xapp. xunfold Heap. unfold Contents. xsimpl*.
+Qed.
+
+Hint Extern 1 (RegisterSpec create) => Provide Triple_create.
+
+Lemma Triple_is_empty : forall p E,
+  SPEC (is_empty p)
+    PRE (p ~> Heap E)
+    POST (fun b => \[b = isTrue (E = \{})] \* p ~> Heap E).
+Proof using.
+  xcf. xunfolds Heap ;=> q. xapp. xapp.
+  xchanges~ Contents_is_empty.
+Qed.
+
+Hint Extern 1 (RegisterSpec (is_empty)) => Provide Triple_is_empty.
+
+Lemma merge_lemma : forall x1 x2 Es1 Es2,
+  Forall (foreach (is_ge x1)) Es1 ->
+  Forall (foreach (is_ge x2)) Es2 ->
+  x1 <= x2 ->
+  Forall (foreach (is_ge x1)) ('{x2} \u list_union Es2 :: Es1).
+Proof using.
+  introv H1 H2 Hg. constructors.
+  { applys foreach_union.
+    { applys* foreach_single. }
+    { applys* foreach_list_union. applys Forall_pred_incl H2.
+      { intros x Hx. applys* foreach_weaken. } } }
+  { eauto. }
+Qed.
+
+Lemma Triple_merge : forall q1 q2 E1 E2,
+  SPEC (merge q1 q2)
+    PRE (q1 ~> Repr E1 \* q2 ~> Repr E2)
+    POST (fun q => q ~> Repr (E1 \u E2)).
+Proof using.
+  xcf. xchange (Repr_eq q1) ;=> x1 q1' Es1 [I11 I12].
+  xchange (Repr_eq q2) ;=> x2 q2' Es2 [I21 I22].
+  xif ;=> C.
+  { xapp. xchange* (Repr_intro q2). xapp. xvals.
+    xchange (Repr_intro q1). { applys* merge_lemma. } xsimpl. substs*. }
+  { xapp. xchange* (Repr_intro q1). xapp. xvals.
+    xchange (Repr_intro q2). { applys* merge_lemma. } xsimpl. substs*. }
+Qed.
+
+Hint Extern 1 (RegisterSpec merge) => Provide Triple_merge.
+
+
+(**
+Lemma Triple_insert : forall p x E,
+  SPEC (insert p x)
+    PRE (p ~> Heap E)
+    POST (fun (_:unit) => p ~> Heap (E \u \{x})).
+Proof using.
+  xcf. xchange Heap_eq ;=> q. xapp ;=> l. xapp ;=> q2.
+  xchange <- Tree_Node. xchange <- Repr_eq. { applys* inv_Node. }
+  rew_listx. xapp. xmatch; simpl.
+  { xpull ;=> ->. xapp. xchanges* Heap_Nonempty. }
+  { xapp ;=> r. xapp. xchanges* Heap_Nonempty. }
+Qed.
+
+Hint Extern 1 (RegisterSpec insert) => Provide Triple_insert.
+
+Lemma Triple_merge_pairs : forall ns l Es,
+  ns <> nil ->
+  Forall2 inv ns Es ->
+  SPEC (merge_pairs l)
+    PRE (l ~> MListOf Tree ns)
+    POST (fun q => q ~> Repr (list_union Es)).
+Proof using.
+  intros ns. induction_wf IH: list_sub ns; introv N Is.
+  xcf. xapp~ ;=> q1 n1 ns' ->. inverts Is as I1 Is. rename r into Es'.
+  xif ;=> C.
+  { subst. inverts Is. rew_listx. xval. xchanges* <- Repr_eq. }
+  { xapp~ ;=> q2 n2 ns'' ->. inverts Is as I2 Is. rename r into Es''.
+    do 2 xchange* <- Repr_eq. xapp ;=> r. xif ;=> C'.
+    { subst. inverts Is. rew_listx. xval. xsimpl. }
+    { xapp* ;=> r'. xapp ;=> r''. rew_listx. xsimpl*. } }
+Qed.
+
+Hint Extern 1 (RegisterSpec merge_pairs) => Provide Triple_merge_pairs.
+
+Lemma Triple_pop_min : forall p E,
+  E <> \{} ->
+  SPEC (pop_min p)
+    PRE (p ~> Heap E)
+    POST (fun x => \exists E', \[min_of E x /\ E = \{x} \u E'] \* p ~> Heap E').
+Proof using.
+  introv HE. xcf. xchange Heap_eq ;=> c. xapp.
+  destruct c as [|q]; simpl; xpull.
+  xchange Repr_eq ;=> [x hs] I. invert I ;=> ? ? ? ? Is Ks Eq -> -> ->.
+  xchange Tree_Node ;=> l. xmatch. xapp. xapp. xapp.
+  xseq (fun (_:unit) => \exists E', \[E = '{x} \u E'] \* p ~> Heap E' \* \GC).
+  { xif ;=> C2.
+    { subst. inverts Is. inverts Ks. rew_listx. xapp. xchanges* Heap_Empty. }
+    { xapp. xapp* ;=> r. xapp. xchange Heap_Nonempty. xsimpl*. } }
+  { xpull ;=> E' ->. xval. xsimpl. split~. { rewrite Eq. applys~ pop_min_lemma. } }
+Qed.
+
+Hint Extern 1 (RegisterSpec pop_min) => Provide Triple_pop_min.
+
+*)
+
+
+
+
+
+End Alternative.
+
+
+
+(* ********************************************************************** *)
+(* ********************************************************************** *)
+(* ********************************************************************** *)
+(** * Representation and lemmas *)
 
 
 (* ******************************************************* *)
@@ -54,23 +374,6 @@ Definition heap := option node.
 
 Instance Inhab_heap : Inhab heap.
 Proof using. applys Inhab_of_val (@None node). Qed.
-
-(** Auxiliary definition for specifications *)
-
-Definition min_of (E:elems) (x:elem) : Prop :=
-  x \in E /\ forall_ y \in E, x <= y.
-
-(** Auxiliary definition for stating invariants follow. *)
-
-(** [is_ge x] is a predicate that characterizes items no less than [x] *)
-
-Definition is_ge (x y:elem) : Prop :=
-  x <= y.
-
-(** [list_union Es] computes the iterated union of the multisets in the list [Es] *)
-
-Definition list_union (Es:list elems) : elems :=
-  LibList.fold_right union \{} Es.
 
 (** [inv n E] relates a tree node [n] with the multiset [E] made of
     the items that the tree contains *)
@@ -128,48 +431,6 @@ Implicit Types hs : list node.
 Implicit Types E : elems.
 Implicit Types Es : list elems.
 
-(** Normalization lemmas for [list_union] *)
-
-Lemma list_union_nil :
-  list_union (@nil elems) = \{}.
-Proof using. auto. Qed.
-
-Lemma list_union_cons : forall E Es,
-  list_union (E::Es) = E \u list_union Es.
-Proof using. auto. Qed.
-
-(** Hints *)
-
-Hint Rewrite list_union_nil list_union_cons : rew_listx.
-Hint Rewrite (@union_empty_r elems _ _ _) (@union_empty_l elems _ _ _) : rew_listx.
-Hint Extern 1 (_ < _) => simpl; math.
-Hint Extern 1 (_ <= _) => simpl; math.
-Hint Extern 1 (_ = _ :> multiset _) => rew_listx; multiset_eq.
-Hint Extern 1 (_ \in _) => multiset_in.
-Hint Constructors Forall Forall2 list_sub.
-Hint Unfold is_ge.
-
-(** Lemmas to manipulate the invariant [Forall (foreach (is_ge x)) Es] *)
-
-Lemma Forall_foreach_is_ge_inv : forall x y Es,
-  Forall (foreach (is_ge x)) Es ->
-  y \in list_union Es ->
-  x <= y.
-Proof using.
-  introv M Hy. unfolds list_union. induction M; rew_listx in *.
-  { multiset_in Hy. }
-  { multiset_in Hy. { applys* H. } { applys* IHM. } }
-Qed.
-
-Lemma foreach_list_union : forall P Es,
-  Forall (foreach P) Es ->
-  foreach P (list_union Es).
-Proof using.
-  introv M. induction M.
-  { applys foreach_empty. }
-  { unfold list_union; rew_listx. applys* foreach_union. }
-Qed.
-
 (** Key auxiliary lemmas for the verification proofs
     (both for the functional version and the imperative version) *)
 
@@ -193,7 +454,7 @@ Proof using.
     { applys foreach_union.
       { applys* foreach_single. }
       { applys* foreach_list_union. applys Forall_pred_incl Ks1.
-        { intros x Hx. applys* foreach_weaken. { intros y Hy. unfolds* is_ge. } } } }
+        { intros x Hx. applys* foreach_weaken. } } }
     { eauto. } }
   { autos*. }
 Qed.
@@ -220,7 +481,6 @@ Qed.
 
 (** [q ~> Tree n] is a notation for [Tree n q]. It relates a pointer [q] with the
     functional tree structure [n] that it represents in memory *)
-
 
 Fixpoint Tree (n:node) (q:loc) { struct n } : hprop :=
   match n with
@@ -407,4 +667,5 @@ Proof using.
 Qed.
 
 Hint Extern 1 (RegisterSpec pop_min) => Provide Triple_pop_min.
+
 
